update

IntervalLists.thy
@@ -15,27 +15,77 @@ fun fusion :: "intvl \<Rightarrow> intvl \<Rightarrow>intvl" where
 
 
 fun inv' :: "nat \<Rightarrow> intvl list \<Rightarrow> bool" where
-"inv' n [] = False"
-|"inv' n [Bd x y] = (if n<x then True else False)"
-|"inv' n [Ub x] = (if n<x then True else False)"
-| " inv' a (Ub vb # v # vc) = (if a<vb then inv' vb (v#vc) else False)"
-|"inv' a (Bd va vd # vb # vc) = (if a<va then inv' vd (vb#vc) else False)"
+"inv' n [] = True"
+| " inv' a (Ub x# v) = ((v=[])\<and>(a\<le>x))"
+|"inv' a ((Bd x y)#v) =((x\<le>y)\<and>(a\<le>x)\<and>(inv' (y+2) (v)))"
 
 definition inv where "inv\<equiv>inv' 0"
 
 fun set_of :: "intvl list \<Rightarrow> nat set" where 
 "set_of [] = {}"
-|"set_of [Bd x y] = {x..y}"
-|"set_of [Ub x] = {x..}"
-|"set_of (Ub vb # v # vc) = {vb..} \<union> set_of (v#vc)"
-|"set_of (Bd va vd # vb # vc) = {va..vd} \<union> set_of (vb#vc)"
+|"set_of (Ub vb # vc) = {vb..} \<union> set_of (vc)"
+|"set_of (Bd va vd # vc) = {va..vd} \<union> set_of (vc)"
 
 fun add :: "nat \<Rightarrow> intvl list \<Rightarrow> intvl list" where
 "add n [] = [Bd n n]"
 |"add n [Bd x y] = (if n+1=x then [Bd n y] else (if n+1<x then (Bd n n)#[Bd x y] else (if n=y+1 then [Bd x n] else (if n>y+1 then [Bd x y]@[Bd n n] else [Bd x y]))))"
-|"add a (Ub vb # va) = (if a+1=vb then (Ub a)#va else (if a>vb then (Ub vb # va) else (Bd a a)#(Ub vb # va) ))"
-|"add a (Bd va vd # vb # vc) = (if a+1<va then (Bd a a)#(Bd va vd # vb # vc) else (if a+1=va then (Bd a vd # vb # vc) else (if a=vd+1 then(if (first_term vb)=a then (fusion (Bd va vd) vb )#vc else (Bd va a # vb # vc))else (Bd va vd)#(add a (vb # vc)) )))"
+|"add a (Ub vb # va) = (if a+1=vb then (Ub a)#va else (if a\<ge>vb then (Ub vb # va) else (Bd a a)#(Ub vb # va) ))"
+|"add a (Bd va vd # vb # vc) = (if a+1<va then (Bd a a)#(Bd va vd # vb # vc) else (if a+1=va then (Bd a vd # vb # vc) else (if a=vd+1 then(if ((first_term vb)=a+1) then (fusion (Bd va vd) vb )#vc else (Bd va a # vb # vc))else (Bd va vd)#(add a (vb # vc)) )))"
 
+value "add (19::nat) [(Bd 0 0),(Bd 5 6),(Bd 8 9),(Bd 11 18),(Ub 20)]"
+
+value "add (0::nat) [Bd 0 0, Bd 1 1]"
+
+lemma lemma1:"inv [u]\<Longrightarrow>(first_term u) = y+2 \<Longrightarrow> x\<le>y \<Longrightarrow> set_of ([fusion (Bd x y) u ]) = (set_of [Bd x y]) \<union> {y+1}  \<union>   set_of [u] "
+ proof (cases u)
+   case (Bd x11 x12)
+   assume "inv [u]" and"(first_term u) = y+2"and" x\<le>y"
+   with Bd 
+ show ?thesis by (auto simp:inv_def)
+next
+  case (Ub x2)
+assume "inv [u]" and"(first_term u) = y+2"and" x\<le>y"
+   with Ub
+ show ?thesis by (auto simp:inv_def)
+qed
+
+
+
+theorem "(inv' c  xs) \<Longrightarrow> (a\<ge>c) \<Longrightarrow> set_of (add a xs) = {a} \<union> set_of xs"
+proof (induction xs arbitrary: a c rule: add.induct )
+  case (1 n)
+  then show ?case  by (auto  split :  if_splits)
+next
+  case (2 n x y)
+  then show ?case  by (auto  split :  if_splits simp:inv_def)
+next
+  case (3 a vb va)
+  then show ?case by (auto  split :  if_splits simp:inv_def)
+next
+  case (4 a va vd vb vc)
+  then show ?case apply (auto  split :  if_splits simp:inv_def lemma1)
+qed
+
+theorem "(a\<ge>c)\<and> inv' c xs \<Longrightarrow> inv' c (add a xs)"
+proof (induction a xs arbitrary: c rule: add.induct )
+  case (1 n)
+  then show ?case by (auto  split :  if_splits)
+next
+  case (2 n x y)
+  then show ?case by (auto  split :  if_splits)
+next
+  case (3 a vb va)
+  then show ?case by (auto  split :  if_splits)
+next
+  case (4 a va vd vb vc)
+  show ?case
+  proof (cases vb)
+  case (Bd l r)
+  with 4 show ?thesis apply (auto  split : if_splits )
+qed
+
+
+qed
 
 
 
